Makefile
@@ -764,7 +764,7 @@ dist/mozilla/Makefile.basic: E_HASH_BUNDLE =
 dist/mozilla/Makefile.basic: MERKLE_BUNDLE = -bundle MerkleTree.*
 dist/mozilla/Makefile.basic: CTR_BUNDLE =
 dist/mozilla/Makefile.basic: SHA3_BUNDLE = -bundle Hacl.SHA3
-dist/mozilla/Makefile.basic: HASH_BUNDLE = -bundle Hacl.Hash.*,Hacl.HKDF,Hacl.HMAC
+dist/mozilla/Makefile.basic: HASH_BUNDLE = -bundle Hacl.Hash.*,Hacl.HKDF,Hacl.HMAC,Hacl.HMAC_DRBG
 dist/mozilla/Makefile.basic: FRODO_BUNDLE = -bundle Hacl.Frodo.*,Hacl.SHA3,Hacl.Keccak,Frodo.Params
 dist/mozilla/Makefile.basic: \
   BUNDLE_FLAGS += \
